workloads/Coq/STLCProplang/Strategies/NewGenerator.v
@@ -158,7 +158,7 @@ Definition test_prop_SinglePreserve   :=
   @Predicate (Expr · ∅) Z
   (fun '(e, tt) => (prop_SinglePreserve e, 0%Z))).
 
-Definition test_prop_SinglePreserve_runner := (targetLoop number_of_trials test_prop_SinglePreserve (DynamicResettingSingletonPool.(mkPool) tt) HillClimbingUtility).
+Definition test_prop_SinglePreserve_runner := (runLoop number_of_trials test_prop_SinglePreserve).
 
 (*! QuickProp test_prop_SinglePreserve_runner. *)
   
@@ -168,7 +168,7 @@ Definition test_prop_MultiPreserve   :=
   @Predicate (Expr · ∅) Z
   (fun '(e, tt) => (prop_MultiPreserve e, 0%Z))).
 
-Definition test_prop_MultiPreserve_runner := (targetLoop number_of_trials test_prop_MultiPreserve (DynamicResettingSingletonPool.(mkPool) tt) HillClimbingUtility).
+Definition test_prop_MultiPreserve_runner := (runLoop number_of_trials test_prop_MultiPreserve).
 
 (*! QuickProp test_prop_MultiPreserve_runner. *)
 (*
